HelloTypeSystem/Meta/ML3.lean
@@ -1,1 +1,2 @@
 import «HelloTypeSystem».Meta.ML3.Eval
+import «HelloTypeSystem».Meta.ML3.Typing
